
\documentclass{exam}

\usepackage{graphicx}
\usepackage[fleqn]{amsmath}
\usepackage{unitsdef} 
\usepackage{cancel}
\usepackage{float}
\usepackage{mdwlist}
\usepackage{booktabs}
\usepackage{cancel}
\usepackage{polynom}
\usepackage{caption}
\usepackage{fullpage}
\usepackage{enumerate}
% \usepackage{parskip}

% \newcommand{\degree}{\ensuremath{^\circ}} 
\everymath{\displaystyle}

\newunit{\inch}{in}
\newunit{\foot}{ft}
\newunit{\cemtimeter}{cm}

% \begin{figure}[H]
%   \centering
%   \includegraphics[scale=.3]{question7.eps}
%   \caption*{Question 7}
% \end{figure}

% \begin{tabular}{cc}
% \toprule
% period & amplitude \\
% \midrule
%   $\pi$ & $2$ \\
% \bottomrule
% \end{tabular}

\printanswers

\ifprintanswers 
\usepackage{2in1, lscape} 
\fi

\title{Math 263B \\ Homework Thirteen}
\date{December 13, 2012}

\begin{document}

\maketitle

\section{Homework}

\begin{itemize*}
  \item Read Section 7.4-7.5
  \item pp 370-372: 1-8, 13-31
  \item pp 377-379: 1-2, 5-8, 11, 13
\end{itemize*}

\ifprintanswers
\pagebreak
\fi

\section{Extra Credit}
page 371, problem 44

\ifprintanswers
\begin{solution}
Solve for x:
\begin{align*}
  y &= \frac{a^x - 1}{a^x + 1} \\
  a^x &= \frac{y + 1}{1 - y} \\
  x &= \log_a \left( \frac{y + 1}{1 - y} \right) \\
\\
  f^{-1}(x) &= \log_a \left( \frac{x + 1}{1 - x} \right) \\
\end{align*}

check:
\begin{align*}
  f(f^{-1}(x)) &= \frac{\cfrac{x + 1}{1 - x} - 1}{\cfrac{x + 1}{1 - x} + 1} = x \\
  f^{-1}(f(x)) &= \log_a \left( \frac{\left( \cfrac{a^x - 1}{a^x + 1} + 1 \right)}{\left(1 - \cfrac{a^x - 1}{a^x + 1} \right)} \right) = x \\
\end{align*}

\end{solution}

\section{Section 7.4}

\begin{description}
\item[1]
\begin{align*}
  x &= \log_2 8 \\
  x &= 3 \\
\end{align*}

\item[2]
\begin{align*}
  \log_5 x &= 2 \\
  x &= 25 \\
\end{align*}

\item[3]
\begin{align*}
  \log_4 x &= \frac{3}{2} \\
  x &= 4^{3/2} \\
    &= 8
\end{align*}

\item[4]
\begin{align*}
  \log_x 64 &= 4 \\
  x^4 &= 64 \\
  x  &= \sqrt[4]{64}
\end{align*}

\item[5]
\begin{align*}
  2 \log_9 \left( \frac{x}{3} \right) &= 1 \\
  \log_9 \left( \frac{x}{3} \right) &= \frac{1}{2} \\
  \frac{x}{3} &= 9^{1/2} \\
%  \frac{x}{3} &= 3 \\
  x &= 9 \\
\end{align*}

\item[6]
\begin{align*}
  \log_4 \left( \frac{1}{2x} \right) &= 3 \\
  \frac{1}{2x} &= 4^3 \\
  x &= \frac{1}{128} \\
\end{align*}

\item[7]
\begin{align*}
  \log_2 (x + 3) - \log_2 x &= 2 \\
  \log_2 \left( \frac{x + 3}{x} \right) &= 2 \\
  \frac{x + 3}{x} &= 2^2 \\
  % x + 3 &= 4x \\
  x &= 1 \\
\end{align*}

\item[8]
\begin{align*}
  \log_5 (x + 3) - \log_5 x &= 1 \\
  \log_5 \left( \frac{x + 3}{x} \right) &= 1 \\
  \frac{x + 3}{x} &= 4 \\
  x + 3 &= 5x \\
  x &= \frac{3}{4} \\
\end{align*}

\item[13]
\begin{align*}
  2^x &= 17 \\
  x &= \log_2 17 \\
    &= \frac{\ln 17}{\ln 2} \\
    &\approx 4.0875 \\
\end{align*}

\item[14]
\begin{align*}
  5^z &= 13 \\
  z &= \log_5 13 \\
    &= \frac{\ln 13}{\ln 5} \\
    &\approx 1.5937 \\
\end{align*}

\item[15]
\begin{align*}
  5^{2s - 3} &= 4 \\
  2s - 3 &= \log_5 4 \\
  2s &= 3 + \log_5 4 \\
  s &= \frac{3 + \log_5 4}{2} \\
    &\approx 1.9307 \\
\end{align*}

\item[16]
\begin{align*}
  12^{1/(\theta - 1)} &= 4 \\
  \frac{1}{\theta - 1} &= \log_12 4 \\
  \theta - 1 &= \frac{1}{\log_12 4} \\
  \theta &= 1 + \frac{1}{\log_12 4} \\
         &\approx 2.7925 \\
\end{align*}

\item[17]
\begin{align*}
  D_x 6^{2x} &= 6^{2x} \cdot \ln 6 \cdot 2
\end{align*}

\item[18]
\begin{align*}
  D_x 3^{2x^2 - 3x} &= 3^{2x^2 - 3x} \cdot (4x - 3)
\end{align*}

\item[19]
\begin{align*}
  D_x \log_3 e^x &= D_x x \log_3 e \\
  &= \log_3 e \\
  &= \frac{\ln e}{\ln 3} \\
  &= \frac{1}{\ln 3} \\
\end{align*}

\item[20]
\begin{align*}
  D_x \log_{10} (x^3 + 9) &= \frac{3x^2}{\ln 10 \cdot (x^3 + 9)}
\end{align*}

\item[21]
\begin{align*}
  D_x \left[ 3^x \ln(x + 5) \right] &= \frac{3^x}{x + 5} + \ln(x + 5) \cdot 3^x \cdot \ln 3 \\
  &= 3^x \left( \frac{1}{x + 5} + \ln 3 \cdot \ln(x + 5) \right) \\
\end{align*}

\item[22]
\begin{align*}
  D_{\theta} \sqrt{ \log 3^{\theta^2 - \theta}} &=  D_{\theta} [ (\log 3^{\theta^2 - \theta})^{1/2} ] \\
    &= \frac{1}{2} \cdot [ \log (3^{\theta^2 - \theta}) ]^{-1/2} \cdot D_{\theta} \log \left(3^{\theta^2 - \theta}\right) \\
    &= \frac{1}{2 \sqrt{ \log 3^{\theta^2 - \theta}}} \cdot  D_{\theta} [  (\theta^2 - \theta) \cdot \log 3 ] \\
    &= \frac{\log 3 \cdot D_{\theta} (\theta^2 - \theta)}{2 \sqrt{\log \left(3^{\theta^2 - \theta}\right)}}  \\
    &= \frac{\log 3 \cdot (2\theta - 1)}{2 \sqrt{\log \left(3^{\theta^2 - \theta}\right)}}  \\
\end{align*}

\item[23]
\begin{align*}
  u &= x^2 \\
  du &= 2 x \, dx
\\
  \int x 2^{x^2} \, \mathrm{d}x &= \frac{1}{2} \int 2^u \, \mathrm{d}u \\
  &= \frac{1}{2} \left( \frac{2^u}{\ln 2} + C \right) \\
  &= \frac{2^u}{2 \cdot \ln 2} + C \\
  &= \frac{2^{x^2}}{2 \cdot \ln 2} + C \\
\end{align*}

check: $D_x \left( \frac{2^{x^2}}{2 \cdot \ln 2} \right) = x 2^{x^2}$

\item[24]
\begin{align*}
  u &= 5x - 1 \\
  du &= 5 \, dx
\\
  \int 10^{5x - 1} \, \mathrm{d}x &= \frac{1}{5} \int 10^u \, \mathrm{d}u \\
  &= \frac{10^u}{5 \cdot \ln 10} + C \\
  &= \frac{10^{5x - 1}}{5 \cdot \ln 10} + C \\
\end{align*}

check: $D_x \left( \frac{10^{5x - 1}}{5 \ln 10} \right) = 10^{5x - 1}$

\item[25]
\begin{align*}
  u &= x^{1/2} \\
  du &= \frac{dx}{2 \sqrt{x}} \\
  u(1) &= 1 \\
  u(4) &= 2 \\
\\
  \int_1^4 \frac{5^{\sqrt{x}}}{\sqrt{x}} \, \mathrm{d}x &= 2 \int_1^2 5^u \, \mathrm{d}u \\
  &= \frac{2 \cdot 5^u}{\ln 5} \bigg|_1^2 \\
  &= \frac{40}{\ln 5} \\
\end{align*}

\item[26]
\begin{align*}
  u &= 3x \\
  du &= 3 \, dx\\
  u(0) &= 0 \\
  u(1) &= 3 \\
\\
  \int_0^1 (10^{3x} + 10^{-3x} \, \mathrm{d}x &= \frac{1}{3} \int_0^3 (10^u + 10^{-u} \, \mathrm{d}u \\
  &= \frac{1}{3 \cdot \ln 10} \cdot \left(10^u + 10^{-u} \right|_0^3 \\
  &= \frac{1000.001}{3 \cdot \ln 10} \\
\end{align*}

\item[27]
\begin{align*}
  y &= 10^{x^2} + (x^2)^{10} \\
    &= 10^{x^2} + x^{20} \\
  y' &= 10^{x^2} \cdot \ln 10 \cdot 2x + 20x^{19} \\
\end{align*}

\item[28]
\begin{align*}
  y &= \sin^2 x + 2^{\sin x} \\
  y' &= 2 \sin x \cos x + 2^{\sin x} \cdot \ln 2 \cdot \cos x \\
\end{align*}

\item[29]
\begin{align*}
  y &= x^{\pi + 1} + (\pi + 1)^x \\
  y' &= (\pi + 1)x^{\pi} + (\pi + 1)^x \ln(\pi + 1) \\
\end{align*}

\item[30]
\begin{align*}
  y &= 2^{e^x} + (2^e)^x \\
    &= 2^{e^x} + 2^{ex} \\
  y' &= 2^{e^x} \cdot \ln 2 \cdot e^x + 2^{ex} \cdot \ln 2 \cdot e \\
     &= e \ln 2 (2^{e^x} \cdot e^{x - 1} + 2^{ex} ) \\
\end{align*}

\item[31]
\begin{align*}
  y &= (x^2 + 1)^{\ln x} \\
  \ln y &= \ln (x^2 + 1)^{\ln x} \\ 
        &= \ln x \cdot \ln (x^2 + 1) \\
  \frac{y'}{y} &= \frac{\ln(x^2 + 1)}{x} + \frac{2x \ln x}{x^2 + 1} \\
  y' &= (x^2 + 1)^{\ln x} \cdot \left( \frac{\ln(x^2 + 1)}{x} + \frac{2x \ln x}{x^2 + 1} \right) \\
\end{align*}

\end{description}

\section{Section 7.5}
\begin{description}

\item[1]
\begin{align*}
  \frac{dy}{dx} &= -6y \\
  \frac{1}{y} \, dy &= -6 dx \\
  \int \frac{1}{y} \, \mathrm{d}y &= -6 \int  \, \mathrm{d}x \\
  \ln y &= -6x + C \\
  e^{\ln y} &= e^{-6x + C} \\
  y &= e^{-6x} \cdot e^C \\
    &= D e^{-6x} \\
\end{align*}
find $D$ using the initial condition of $y(0) = 4$:
\begin{align*}
  4 &= D e^0 \\
  D &= 4 \\
\end{align*}
the final equation is:
\[
  y = 4e^{-6x}
\]
check:
\[
  D_x 4e^{-6x} = -6 \cdot 4 e^{-6x} = -6 y
\]

\item[2]
\begin{align*}
  \frac{dy}{dx} &= 6y \\
  \frac{1}{y} \, dy &= 6 dx \\
  \int \frac{1}{y} \, \mathrm{d}y &= 6 \int  \, \mathrm{d}x \\
  \ln y &= 6x + C \\
  e^{\ln y} &= e^{6x + C} \\
  y &= e^{6x} \cdot e^C \\
    &= D e^{-6x} \\
\end{align*}
find $D$ using the initial condition of $y(0) = 1$:
\begin{align*}
  1 &= D e^0 \\
  D &= 1 \\
\end{align*}
the final equation is:
\[
  y = e^{6x}
\]
check:
\[
  D_x e^{6x} = 6 \cdot e^{6x} = 6y
\]

\item[5]
Here are the facts from the problem:
\begin{itemize*}
  \item P(0) = 10,000 bacteria
  \item P(10) = 20,000 bacteria
\end{itemize*}

The equation will look like: $P = P_0 e^{kt}$, so we need to find $k$ and then plug 25 into the resulting equation:
\begin{align*}
  P &= P_0 e^{kt} \\
  20,000 &= 10,000 e^{10k} \\
  2 &= e^{10k} \\
  \ln 2 &= 10 k \\
  k &= \frac{\ln 2}{10} \\
    &\approx 0.069315 \\
\end{align*}
The equation is:
\[
  P(t) = 10,000 e^{0.069315 t}
\]
After 25 days:
\[
  P(25) = 10,000 e^{0.069315 \cdot 25} = 56,568 \text{ bacteria}
\]

\item[6]
The population doubles every 10 days because it starts out at 10,000 and 10 days later is 20,000.  The population after
20 days should be 40,000.  We can verify this with the equation:
\[
  P(20) = 10,000 e^{0.069314 \cdot 20} = 40,000 \text{ bacteria}
\]

\item[7]
When the population has tripled, there are 30,000 bacteria.  We need to solve for $t$:
\begin{align*}
  30,000 &= 10,000 e^{0.069314 t} \\
  3      &= e^{0.069314 t} \\
  \ln 3  &= 0.069314 t \\
  t      &= \frac{\ln 3}{0.069314} \\
         &= 15.85 \text{ days} \\
\end{align*}

This seems reasonable, since we know the population doubled after 10 days and quadrupled after 20 days.

\item[8]
If we let 1790 be year zero and do all the calculations in millions of people:
\begin{itemize*}
  \item P(0) = 4
  \item P(170) = 180
\end{itemize*}

The equation will look like: $P = P_0 e^{kt}$, so we need to find $k$ and then plug 230 into the resulting equation:
\begin{align*}
  P &= P_0 e^{kt} \\
  180 &= 4 e^{170k} \\
  45 &= e^{170k} \\
  \ln 45 &= 170k \\
    &= \frac{\ln 45}{170} \\
    &\approx 0.0223921 \\
\end{align*}
The equation is:
\[
  P(t) = 4 e^{0.0223921 t}
\]
After 230 years:
\[
  P(230) = 4 e^{0.0223921 \cdot 230} = 690 \text{ million}
\]

\item[11]
10 grams turns into 5 grams after 700 years.  We can use this to find $k$:
\begin{align*}
  x           &= x_0 e^{kt} \\
  5           &= 10 e^{700 k} \\
  \frac{1}{2} &= e^{700 k} \\
  - \ln 2    &= 700 k \\
  k &= - \frac{\ln 2}{700} \\
    &\approx -9.9021 \cdot 10^{-4} \\
\end{align*}

The equation is:
\[
  x = 10 e^{-9.9021 \cdot 10^{-4} \cdot t}
\]

After 300 years:
\[
  x = 10 e^{-9.9021 \cdot 10^{-4} \cdot 300} \approx 7.43 \gram
\]

\item[13]
1 grams turns into $\frac{1}{2}$ gram after 5730 years.  We can use this to find $k$:
\begin{align*}
  \frac{1}{2} &= e^{5730k} \\
  - \ln 2    &= 5730 k \\
   k &= - \frac{\ln 2}{5730} \\
    &= -1.2097 \cdot 10^{-4} \\
\end{align*}

The equation is:
\[
  x = x_0 e^{-1.2097 \cdot 10^{-4} \cdot t}
\]

We need to find the time when the amount is $0.7 x_0$:
\begin{align*}
  0.7 x_0  &= x_0 e^{-1.2097 \cdot 10^{-4} \cdot t} \\
  0.7      &= e^{-1.2097 \cdot 10^{-4} \cdot t} \\
  \ln 0.7  &= -1.2097 \cdot 10^{-4} \cdot t \\
  t        &= \frac{\ln 0.7}{-1.2097 \cdot 10^{-4}} \\
           &\approx 2948 \text{ years} \\
\end{align*}


\end{description}
\else

% Law never made men a whit more just; and, by means of their respect for it, even the well-disposed are daily made the
% agents of injustice (Thoreau)

\vspace{9 cm} 

{\em I heartily accept the motto, ``That government is best which governs least''; and I should like to see it acted up
  to more rapidly and systematically. Carried out, it finally amounts to this, which also I believe---``That government
  is best which governs not at all''; and when men are prepared for it, that will be the kind of government which they
  will have.}

\vspace{0.1 cm}
\hspace{0.5 cm} --Henry David Thoreau

\fi

\end{document}

