
\documentclass{exam}

\usepackage{fullpage}
\usepackage{enumerate}
\usepackage{siunitx} 
\usepackage{graphicx}
\usepackage[fleqn]{amsmath}
\usepackage{cancel}
\usepackage{polynom}
\usepackage{float}
\usepackage{mdwlist}
\usepackage{booktabs}
\usepackage{cancel}
\usepackage{polynom}
\usepackage{caption}

\newcommand{\degree}{\ensuremath{^\circ}} 
\everymath{\displaystyle}

% \begin{figure}[H]
%   \centering
%   \includegraphics[scale=.3]{question7.eps}
%   \caption*{Question 7}
% \end{figure}

% \begin{tabular}{cc}
% \toprule
% period & amplitude \\
% \midrule
%   $\pi$ & $2$ \\
% \bottomrule
% \end{tabular}

% \textwidth 6.5 in

\printanswers

\ifprintanswers 
\usepackage{2in1, lscape} 
\fi

\title{Math 263a \\ Homework Three}
\date{February 1, 2012}

\begin{document}

\maketitle

\section{Homework}

\begin{itemize*}
  \item Read Section 2.4-2.5
  \item pp 70-71: 5-8, 13-16, 27-28, 30
  \item pp 78-79: 2, 7-12
\end{itemize*}

\section{Extra Credit}
\begin{itemize*}
\item pp 70-71: 34 and 36
% \item pp 78: 27
\end{itemize*}

\ifprintanswers

\begin{description}
\item[34]
\begin{align*}
  \lim_{x \to 0} \frac{\sqrt{x+2} - \sqrt{2}}{x} 
    &= \lim_{x \to 0} \left( \frac{\sqrt{x+2} - \sqrt{2}}{x} \right) \left( \frac{\sqrt{x+2} + \sqrt{2}}{\sqrt{x+2} + \sqrt{2}} \right) \\
    &= \lim_{x \to 0} \frac{x+2 - 2}{x(\sqrt{x+2} + \sqrt{2})}  \\
    &= \lim_{x \to 0} \frac{x}{x(\sqrt{x+2} + \sqrt{2})} \\
    &= \lim_{x \to 0} \frac{1}{\sqrt{x+2} + \sqrt{2}} \\
    &= \frac{1}{2 \sqrt{2}} \\
    &= \frac{\sqrt{2}}{4} \\
\end{align*}
\end{description}



\section{Section 2.4}
\begin{description}
\item[5]
\[
  \lim_{t \to -1} \frac{1-2t}{\sqrt{3t + 21}} = \frac{1 + 2}{\sqrt{-3 + 21}} = \frac{3}{\sqrt{18}} = \frac{\sqrt{2}}{2}
\]

\item[6]
\[
  \lim_{t \to -1} \frac{\sqrt{1-2t}}{(3t + 2)^3} = \frac{\sqrt{3}}{(-1)^3} = - \sqrt{3}
\]

\item[7]
\begin{align*}
  \lim_{x \to 2} \frac{x^2 - 4}{x-2} &=   \lim_{x \to 2} \frac{(x+2)(x-2)}{x-2} \\
  &= \lim_{x \to 2} x+2 \\
  &= 4 \\
\end{align*}

\item[8]
\begin{align*}
  \lim_{t \to -7} \frac{t^2 + 4t - 21}{t+7} &= \lim_{t \to -7} \frac{(t-3)(t+7)}{t+7} \\
  &= \lim_{t \to -7} t-3 \\
  &= -10 \\
\end{align*}

\item[13]
\begin{align*}
  \lim_{t \to 2} \frac{\sqrt{(t+4)(t-2)^4}}{(3t-6)^2} &= \lim_{t \to 2} \frac{(t-2)^2\sqrt{t+4}}{3^2(t-2)^2} \\
  &= \lim_{t \to 2} \frac{\sqrt{t+4}}{9} \\
  &= \frac{\sqrt{6}}{9} \\
\end{align*}

\item[14]
\begin{align*}
  \lim_{t \to 7} \frac{\sqrt{(t-7)^3}}{t-7} &= \lim_{t \to 7} \frac{(t-7)\sqrt{t-7}}{t-7} \\
  &= \lim_{t \to 7} \sqrt{t-7} \\
  &= 0 \\
\end{align*}

\item[15]
\begin{align*}
   \lim_{x \to 3} \frac{x^4 - 18x^2 + 81}{(x-3)^2} &= \lim_{x \to 3} \frac{(x^2 - 9)^2}{(x-3)^2} \\
   &= \lim_{x \to 3} \frac{(x + 3)^2(x-3)^2}{(x-3)^2} \\
   &= \lim_{x \to 3} (x + 3)^2 \\
   &= 36 \\
\end{align*}

\item[16]
\begin{align*}
   \lim_{u \to 1} \frac{(3u + 4)(2u-2)^3}{(u-1)^2} &=  \lim_{u \to 1} \frac{2^3(3u + 4)(u-1)^3}{(u-1)^2} \\
   &= \lim_{u \to 1} 8 (3u + 4)(u-1) \\  
   &= 0 \\
\end{align*}

\item[27]
\begin{enumerate}[(a)]

\item $\lim_{x \to -3} f(x) = 2$
\item $f(-3) = 1$
\item $f(-1)$ is not defined
\item $\lim_{x \to -1} f(x) = 2.5$

\item $f(1) = 2$
\item $\lim_{x \to 1} f(x)$ is not defined since it the limit is different depending on which direction you approach 1 from.

\item $\lim_{x \to 1^-} f(x) = 2$ 
\item $\lim_{x \to 1^+} f(x) = 1$ 

\end{enumerate}

\item[28]
\begin{enumerate}[(a)]

\item $\lim_{x \to -3} f(x)$ is not defined since the limit is different depending on which direction you approach $-3$ from.
\item $f(-3) = 1$

\item $f(-1) = 1$
\item $\lim_{x \to -1} f(x) = 2$

\item $f(1) = 1$
\item $\lim_{x \to 1} f(x)$ is not defined since the function appears to oscillate between 0.75 and 1.25 when approaching 1
  from the positive side.

\item $\lim_{x \to 1^-} f(x) = 1$ 
\item $\lim_{x \to 1^+} f(x)$ is not defined

\end{enumerate}

\item[30]
\begin{figure}[H]
  \centering
  \includegraphics[scale=.3]{problem_30.eps}
  \caption*{Problem 30}
\end{figure}

\begin{enumerate}[(a)]

\item $\lim_{x \to 1} g(x) = 0$
\item $g(1)$ is not defined

\item $\lim_{x \to 2} g(x) = 1$
\item $\lim_{x \to 2^-} g(x) = 1$

\end{enumerate}

\end{description}

\section{Section 2.5}
\begin{description}

\item[2]

For any $\epsilon$ there is a $\delta$ such that if $|u - b| < \delta$ then $|g(u) - L| < \epsilon$.

\item[7]
To prove: for any $\epsilon$ there is a $\delta$ such that if $|x| < \delta$ then $|2x - 1 + 1| < \epsilon$.

Preliminary Investigation:
\begin{align*}
  |2x - 1 + 1| &< \epsilon \\
  2|x| &< \epsilon \\
  |x| &< \frac{\epsilon}{2} \\
\end{align*}

Select $\delta = \frac{\epsilon}{2}$ and show that if $|x| < \delta$ then $|2x - 1 + 1| < \epsilon$

\begin{itemize}
  \item $|2x - 1 + 1| = 2|x|$
  \item $2|x| < 2 \delta$ since $|x| < \delta$
  \item $2 \delta = 2 \left( \frac{\epsilon}{2} \right) = \epsilon$
\end{itemize}

Putting it all together:
\begin{align*}
  |2x - 1 + 1| = 2|x| &< 2 \delta = 2 \left( \frac{\epsilon}{2} \right) = \epsilon \\
  |2x - 1 + 1| < \epsilon \\
\end{align*}

Therefore, if $|x| < \delta$ then $|2x - 1 + 1| < \epsilon$ when $\delta = \frac{\epsilon}{2}$.

\item[8]
To prove: for any $\epsilon$ there is a $\delta$ such that 
\[
  \text{ if } |x + 21| < \delta \text{ then } |3x - 1 + 64| < \epsilon.
\]

Preliminary Investigation:
\begin{align*}
  |3x - 1 + 64| &< \epsilon \\
  3|x + 21| &< \epsilon \\
  |x + 21| &< \frac{\epsilon}{3} \\
\end{align*}

Select $\delta = \frac{\epsilon}{3}$ and show that if $|x + 21| < \delta$ then $|3x - 1 + 64| < \epsilon$

\begin{itemize}
  \item $|3x - 1 + 64| = 3|x + 21|$
  \item $3|x + 21| < 3 \delta$ since $|x + 21| < \delta$
  \item $3 \delta = 3 \left( \frac{\epsilon}{3} \right) = \epsilon$
\end{itemize}

Putting it all together:
\begin{align*}
  |3x - 1 + 64| = 3|x + 21| &< 3 \delta = 3 \left( \frac{\epsilon}{3} \right) = \epsilon \\
  |3x - 1 + 64| &< \epsilon
\end{align*}

Therefore, if $|x| < \delta$ then $|3x - 1 + 64| < \epsilon$ when $\delta = \frac{\epsilon}{3}$

\item[9]
To prove: For any $\epsilon$ there is a $\delta$ such that 
\[
  \text{if } |x - 5| < \delta \text{ then } \left|\frac{x^2 - 25}{x-5} - 10\right| < \epsilon
\]

Preliminary Investigation:
\begin{align*}
  \left| \frac{x^2 - 25}{x-5} - 10 \right| &< \epsilon \\
  \left| \frac{(x+5)(x-5)}{x-5} - 10 \right| &< \epsilon \\
  |x - 5| &< \epsilon \\
\end{align*}

Select $\delta = \epsilon$ and show that if $|x - 5| < \delta$ then $\left| \frac{x^2 - 25}{x-5} - 10 \right| < \epsilon$

\begin{itemize}
  \item $\left| \frac{x^2 - 25}{x-5} - 10 \right| = \left| x - 5 \right|$
  \item $\left| x - 5 \right| < \delta$
  \item $\delta = \epsilon$
\end{itemize}

Putting it all together:
\begin{align*}
  \left| \frac{x^2 - 25}{x-5} - 10 \right| = | x - 5 | &< \delta = \epsilon \\ 
  \left| \frac{x^2 - 25}{x-5} - 10 \right| &< \epsilon \\ 
\end{align*}

Therefore, if $|x - 5| < \delta$ then $\left| \frac{x^2 - 25}{x-5} - 10 \right| < \epsilon$ when $\delta = \epsilon$.

\pagebreak

\item[10]
To prove: For any $\epsilon$ there is a $\delta$ such that 
\[
  \text{if } |x| < \delta \text{ then } \left|\frac{2x^2 - x}{x} + 1\right| < \epsilon
\]

Preliminary Investigation:
\begin{align*}
  \left|\frac{2x^2 - x}{x} + 1\right| &< \epsilon \\
  |2x - 1 + 1| &< \epsilon \\
  |2x| &< \epsilon \\
  |x| &< \frac{\epsilon}{2} \\
\end{align*}

Select $\delta = \frac{\epsilon}{2}$ and show that if $|x| < \delta$ then $\left|\frac{2x^2 - x}{x} + 1\right| < \epsilon$

\begin{itemize}
  \item $\left|\frac{2x^2 - x}{x} + 1\right| = |2x| = 2|x|$
  \item $2|x| < 2 \delta$ since $|x| < \delta$.
  \item $2 \delta = 2 \left( \frac{\epsilon}{2} \right) = \epsilon$
\end{itemize}

Putting it all together:
\begin{align*}
  \left|\frac{2x^2 - x}{x} + 1\right| = 2|x| &< 2 \delta = 2 \left( \frac{\epsilon}{2} \right) = \epsilon \\ 
  \left|\frac{2x^2 - x}{x} + 1\right| &< \epsilon \\ 
\end{align*}

Therefore, if $|x| < \delta$ then $\left|\frac{2x^2 - x}{x} + 1\right| < \epsilon$ when $\delta = \frac{\epsilon}{2}$.

\pagebreak

\item[11]
To prove: For any $\epsilon$ there is a $\delta$ such that 
\[
  \text{if } |x - 5| < \delta \text{ then } \left|\frac{2x^2 - 11x + 5}{x-5} -9 \right| < \epsilon
\]

Preliminary Investigation:
\begin{align*}
  \left|\frac{2x^2 - 11x + 5}{x-5} -9 \right| < \epsilon \\
  \left|\frac{(2x - 1)(x-5)}{x-5} -9 \right| < \epsilon \\
  |2x - 1 - 9| &< \epsilon \\
  |2x - 10| &< \epsilon \\
  2|x - 5| &< \epsilon \\
  |x - 5| &< \frac{\epsilon}{2} \\
\end{align*}

Select $\delta = \frac{\epsilon}{2}$ and show that if $|x - 5| < \delta$ then 
\[
  \left|\frac{2x^2 - 11x + 5}{x-5} -9 \right| < \epsilon
\]

\vspace{0.2 cm}

\begin{itemize}
  \item $\left|\frac{2x^2 - 11x + 5}{x-5} -9 \right| = 2|x-5|$
  \item $2|x - 5| < 2 \delta$ since $|x - 5| < \delta$.
  \item $2 \delta = 2 \left( \frac{\epsilon}{2} \right) = \epsilon$
\end{itemize}

Putting it all together:
\begin{align*}
  \left|\frac{2x^2 - 11x + 5}{x-5} -9 \right| = 2|x-5| &< 2 \delta = 2 \left( \frac{\epsilon}{2} \right) = \epsilon \\ 
  \left|\frac{2x^2 - 11x + 5}{x-5} -9 \right| &< \epsilon \\ 
\end{align*}

Therefore, if $|x - 5| < \delta$ then $\left|\frac{2x^2 - 11x + 5}{x-5} -9 \right| < \epsilon$ when $\delta = \frac{\epsilon}{2}$.

\item[12]
To prove: For any $\epsilon$ there is a $\delta$ such that 
\[
  \text{if } |x - 1| < \delta \text{ then } | \sqrt{2x} - \sqrt{2} | < \epsilon
\]

Preliminary Investigation:
\begin{align*}
  | \sqrt{2x} - \sqrt{2}| < \epsilon \\
  \left| \sqrt{2x} - \sqrt{2} \left( \frac{\sqrt{2x} + \sqrt{2}}{\sqrt{2x} + \sqrt{2}} \right) \right| < \epsilon \\
  \left| \frac{2x - 2}{\sqrt{2x} + \sqrt{2}} \right| < \epsilon \\
  \left| \frac{2(x - 1)}{\sqrt{2}(x + 1)} \right| < \epsilon \\
  \sqrt{2} \left| \frac{x - 1}{\sqrt{x} + 1} \right| < \epsilon \\
  \\
  \left| \frac{x - 1}{\sqrt{x} + 1} \right| \leq |x - 1| \text{ since } \sqrt{x} \geq 0 \\
  \\
  \sqrt{2} | x - 1| < \epsilon \\
  | x - 1| < \frac{\epsilon}{\sqrt{2}} \\
\end{align*}

Select $\delta = \frac{\epsilon}{\sqrt{2}}$ and show that if $|x - 1| < \delta$ then $\left|\sqrt{2x} - \sqrt{2} \right| < \epsilon$

\vspace{0.2 cm}

\begin{align*}
  | \sqrt{2x} - \sqrt{2}| = \sqrt{2} \left| \frac{x - 1}{\sqrt{x} + 1} \right| &\leq  \sqrt{2} | x - 1| \\
      &< \sqrt{2} \cdot \delta = \sqrt{2} \left( \frac{\epsilon}{\sqrt{2}} \right) = \epsilon \\ 
  | \sqrt{2x} - \sqrt{2}| &< \epsilon \\ 
\end{align*}

Therefore, if $|x - 1| < \delta$ then $| \sqrt{2x} - \sqrt{2}| < \epsilon$ when $\delta = \frac{\epsilon}{\sqrt{2}}$.

\end{description}
\else

\vspace{10 cm}

{\em I can't understand why people are frightened of new ideas. I'm frightened of the old ones.}

\vspace{.2 cm}

\hspace{1 cm} --John Cage

\fi

\end{document}

