\documentclass{exam}

\usepackage{units} 
\usepackage{graphicx}
\usepackage[fleqn]{amsmath}
\usepackage{cancel}
\usepackage{float}
\usepackage{mdwlist}
\usepackage{booktabs}
\usepackage{cancel}
\usepackage{polynom}
\usepackage{caption}
\usepackage{fullpage}
\usepackage{comment}
\usepackage{enumerate}
\usepackage{xfrac}

\newcommand{\dg}{\ensuremath{^\circ}} 
\everymath{\displaystyle}

\printanswers
\excludecomment{comment}

\ifprintanswers 
  \usepackage{2in1, lscape} 
\fi

\author{}
\date{\today}
\title{Math 142 \\ Homework Twelve}

\begin{document}

  \maketitle

  \section{Homework}
  Section 7.1: 

  \section{Extra Credit}
  Section 7.1: 

  \ifprintanswers
    \pagebreak
  \fi

  \section{Review}

  \ifprintanswers
    \section{Section 7.1}
    \begin{description}

      \item[1] 
        \begin{align*}
          \cos t \tan t & = \cos t \cdot \frac{\sin t}{\cos t} \\
                        & = \boxed{ \sin t } \\
        \end{align*}

      \item[2] 
        \begin{align*}
          \cos t \csc t & = \cos t \cdot frac{1}{\sin t} \\
                        & = \boxed{ \cot t } \\
        \end{align*}

      \item[3] 
        \begin{align*}
          \sin \theta \sec \theta & = \sin \theta \cdot \frac{1}{\cos \theta} \\
                                  & = \boxed{ \tan t } \\
        \end{align*}

      \item[4] 
        \begin{align*}
          \tan \theta \csc \theta & = \frac{\sin \theta}{\cos \theta} \cdot \frac{1}{\sin \theta} \\
                                  & = \boxed{ \sec t } \\
        \end{align*}

      \item[5] 
        \begin{align*}
          \tan^2 x - \sec^2 x & = \frac{\sin^2 x}{\cos^2 x} - \frac{1}{\cos^2 x} \\
                              & = \frac{\sin^2 x - 1}{\cos^2 x} \\
                              & = \frac{- \cos^2 x}{\cos^2 x} \\
                              & = \boxed{ -1 } \\
        \end{align*}

      \item[6] 
        \begin{align*}
          \frac{\sec x}{\csc x} & = \frac{\sin x}{\cos x} \\
                                & = \boxed{ \tan x } \\
        \end{align*}

      \item[7] 
        \begin{align*}
          \sin u + \cot u \cos u & = \sin u + \frac{\cos u}{\sin u} \cdot \cos u \\
                                 & = \sin u + \frac{\cos^2 u}{\sin u} \\
                                 & = \frac{\sin^2 u + \cos^2 u}{\sin u} \\
                                 & = \frac{1}{\sin u} \\
                                 & = \boxed{ \csc u } \\
        \end{align*}

      \item[8] 
        \begin{align*}
          \cos^2 \theta \left( 1 + \tan^2 \theta \right) & = \cos^2 \theta \left( 1 + \frac{\sin^2 \theta}{\cos^2 \theta} \right) \\
                                                         & = \cos^2 \theta \cdot \frac{\sin^2 \theta + \cos^2 \theta}{\cos^2 \theta} \\
                                                         & = \boxed{ 1 } \\
        \end{align*}

      \item[9] 
        \begin{align*}
          \frac{\sec \theta - \cos \theta}{\sin \theta} & = \frac{\sfrac{1}{\cos \theta} - \cos \theta}{\sin \theta} \\
                                                        & = \frac{\sfrac{1 - \cos^2 \theta}{\cos \theta}}{\sin \theta} \\
                                                        & = \frac{\sin^2 \theta}{\sin \theta \cos \theta} \\
                                                        & = \frac{\sin \theta}{\cos \theta} \\
                                                        & = \boxed{ \tan \theta } \\
        \end{align*}

      \item[10] 
        \begin{align*}
          \frac{\cot \theta}{\csc \theta - \sin \theta} & = \frac{\sfrac{\cos \theta}{\sin \theta}}{\sfrac{1}{\sin \theta} - \sin \theta} \\
                                                        & = \frac{\cos \theta}{1 - \sin^2 \theta} \\
                                                        & = \frac{\cos \theta}{\cos^2 \theta} \\
                                                        & = \frac{1}{\cos^2 \theta} \\
                                                        & = \boxed{ \sec \theta } \\
        \end{align*}

      \item[11] 
        \begin{align*}
          \frac{\sin x \sec x}{\tan x} & = \frac{\sin x}{\cos x \cdot \sfrac{\sin x}{\cos x}} \\
                                       & = \frac{\sin x}{\sin x} \\
                                       & = \boxed{ 1 } \\
        \end{align*}

      \item[12] 
        \begin{align*}
          \cos^3 x + \sin^2 x \cos x & = \cos x \left( \cos^2 x + \sin^2 x \right) \\
                                     & = \boxed{ \cos x } \\
        \end{align*}

      \item[13] 
        \begin{align*}
          \frac{1 + \cos y}{1 + \sec y} & = \frac{1 + \cos y}{1 + \sfrac{1}{\cos y}} \\
                                        & = \frac{1 + \cos y}{\sfrac{\cos y + 1}{\cos y}} \\
                                        & = \boxed{ \cos y } \\
        \end{align*}

      \item[14] 
        \begin{align*}
          \frac{\tan x}{\sec(-x)}      & = \frac{\tan x}{\sec x} \\
          \frac{\sin x \cos x}{\cos x} & = \boxed{ \sin x } \\
        \end{align*}

      \item[20] 
        \begin{align*}
          \tan x \cos x \csc x & = \frac{\sin x}{\cos x} \cdot \cos x \cdot \frac{1}{\sin x} \\
                               & = \boxed{ 1 } \\
        \end{align*}

      \item[21] 
        \begin{align*}
          \frac{2 + \tan^2 x}{\sec^2 x} - 1 & = \frac{2 + \tan^2 x - \sec^2 x}{\sec^2 x} \\
                                            & = \frac{1}{\sec^2 x} \\
                                            & = \boxed{ \cos^2 x } \\
        \end{align*}

      \item[22] 
        \begin{align*}
          \frac{1 + \cot A}{\csc A} & = \frac{1}{\csc A} + \frac{\cos A \sin A}{\sin A} \\
                                    & = \boxed{ \sin A + \cos A } \\
        \end{align*}

      \item[23] 
        \begin{align*}
          \tan \theta + \cos(- \theta) + \tan(- \theta) & = \tan \theta + \cos \theta - \tan \theta \\
                                                        & = \boxed{ \cos \theta } \\
        \end{align*}

      \item[24] 
        \begin{align*}
          \frac{\cos x}{\sec x + \tan x} & = \frac{\cos x}{\sfrac{1}{\cos x} + \sfrac{\sin x}{\cos x}} \\
                                         & = \frac{\cos^2 x}{1 + \sin x} \cdot \frac{1 - \sin x}{1 - \sin x} \\
                                         & = \frac{\cos^2 x (1 - \sin x)}{1 - \sin^2 x} \\
                                         & = \boxed{ 1 - \sin x } \\
        \end{align*}

      \item[25] 
        \begin{align*}
          \frac{\sin \theta}{\tan \theta} & = \sin \theta \cdot \frac{\cos \theta}{\sin \theta} \\
                                          & = \cos \theta \\
        \end{align*}

      \item[26] 
        \begin{align*}
          \frac{\tan \theta}{\sec \theta} & = \frac{\sin \theta}{\cos \theta} \cdot \cos \theta \\
                                          & = \sin \theta \\
        \end{align*}

      \item[27] 
        \begin{align*}
          \frac{\cos u \sec u}{\tan u} & = \frac{\cos u \cdot \sfrac{1}{\cos u}}{\tan u} \\
                                       & = \frac{1}{\tan u} \\
                                       & = \cot u \\
        \end{align*}

      \item[28] 
        \begin{align*}
          \frac{\cot x \sec x}{\csc x} & = \frac{\cos x}{\sin x} \cdot \frac{1}{\cos} \cdot \sin x \\
                                       & = 1 \\
        \end{align*}

      \item[29] 
        \begin{align*}
          \frac{\tan y}{\csc y} & = \frac{\sin^2 y}{\cos y} \\
                                & = \frac{1 - \cos^2 y}{\cos y} \\
                                & = \sec y - \cos y \\
        \end{align*}

      \item[30] 
        \begin{align*}
          \frac{\cos v}{\sec v \sin v} & = \frac{\cos^2 v}{\sin v} \\
                                       & = \frac{1 - \sin^2 v}{\sin v} \\
                                       & = \csc v - \sin v \\
        \end{align*}

      \item[31] 
        \begin{align*}
          \sin B + \cos B \cot B & = \sin B + \frac{\cos^2 B}{\sin B} \\
                                 & = \frac{\sin^2 B + \cos^2 B}{\sin B} \\
                                 & = \frac{1}{\sin B} \\
                                 & = \csc B \\
        \end{align*}

      \item[32] 
        \begin{align*}
          \cos(-x) - \sin(-x) & = \cos x - (- \sin x) \\
                              & = \cos x + \sin x \\
        \end{align*}

      \item[33] 
        \begin{align*}
          \cot(- \alpha) \cos(- \alpha) + \sin(-\alpha) & = - \cot \alpha \cos \alpha - \sin \alpha \\
                                                        & = - \left( \frac{\cos^2 \alpha}{\sin \alpha} + \sin \alpha \right) \\
                                                        & = - \left( \frac{\cos^2 \alpha + \sin^2 \alpha}{\sin \alpha} \right) \\
                                                        & = - \left( \frac{1}{\sin \alpha} \right) \\
                                                        & = - \csc \alpha \\
        \end{align*}

      \item[34] 
        \begin{align*}
          \csc x [\csc x + \sin(-x)] & = \csc x (\csc x - \sin x) \\
                                     & = \csc^2 x - 1 \\
                                     & = \cot^2 x \\
        \end{align*}

      \item[40] 
        \begin{align*}
          (\sin x + \cos x)^4 & = \left( \sin^2 x + 2 \sin x \cos x + \cos^2 x \right)^2 \\
                              & = ( 1 + 2 \sin x \cos x )^2 \\
        \end{align*}

      \item[41] 
        \begin{align*}
          \frac{\sec t - \cos t}{\sec t} & = 1 - \frac{\cos t}{\sfrac{1}{\cos t}} \\
                                         & = 1 - \cos^2 t \\
                                         & = \sin^2 t \\
        \end{align*}

      \item[42] 
        \begin{align*}
          \frac{1 - \sin x}{1 + \sin x} & = \frac{1 - \sin x}{1 + \sin x} \cdot \frac{1 - \sin x}{1 - \sin x} \\
                                        & = \frac{1 - 2 \sin x + \sin^2 x}{1 - \sin^2 x} \\
                                        & = \frac{1 - 2 \sin x + \sin^2 x}{\cos^2 x} \\
                                        & = \sec^2 x - 2 \sec x \tan x + \tan^2 x \\
                                        & = (\sec x - \tan x)^2 \\
        \end{align*}

      \item[43] 
        \begin{align*}
          \frac{1}{1 - \sin^2 y} & = \frac{1}{\cos^2 y} \\
                                 & = \sec^2 y \\
                                 & = 1 + \tan^2 y \\
        \end{align*}

      \item[44] 
        \begin{align*}
          \csc x - \sin x & = \frac{1}{\sin x} - \sin x \\
                          & = \frac{1 - \sin^2 x}{\sin x} \\
                          & = \frac{\cos^2 x}{\sin x} \\
                          & = \cos x \cot x \\
        \end{align*}

      \item[50] 
        \begin{align*}
          (\tan y + \cot y) \sin y \cos y & = \left( \frac{\sin y}{\cos y} + \frac{\cos y}{\sin y} \right) \sin y \cos y \\
                                          & = \sin^2 y + \cos^2 y \\
                                          & = 1 \\
        \end{align*}

      \item[51] 
        \begin{align*}
          \frac{1 - \cos \alpha}{\sin \alpha} & = \frac{1 - \cos \alpha}{\sin \alpha} \cdot \frac{1 + \cos \alpha}{1 + \cos \alpha} \\
                                              & = \frac{1 - \cos^2 \alpha}{\sin \alpha ( 1 + \cos \alpha ) } \\
                                              & = \frac{\sin^2 \alpha}{\sin \alpha ( 1 + \cos \alpha ) } \\
                                              & = \frac{\sin \alpha}{1 + \cos \alpha } \\
        \end{align*}

      \item[52] 
        \begin{align*}
          \sin^2 \alpha + \cos^2 \alpha + \tan^2 \alpha & = 1 + \tan^2 \alpha \\
                                                        & = \sec^2 \alpha \\
        \end{align*}

      \item[53] 
        \begin{align*}
          \tan^2 \theta - \sin^2 \theta & = \frac{\sin^2 \theta}{\cos^2 \theta} - \sin^2 \theta \\
                                        & = \sin^2 \theta \left( \frac{1}{\cos^2 \theta} - 1 \right) \\
                                        & = \sin^2 \theta \left( \sec^2 \theta - 1 \right) \\
                                        & = \tan^2 \theta \sin^2 \theta \\
        \end{align*}

      \item[54] 
        \begin{align*}
          \cot^2 \theta \cos^2 \theta & = \cot^2 \theta \left( 1 - \sin^2 \theta \right) \\
                                      & = \frac{\cos^2 \theta}{\sin^2 \theta} \left( 1 - \sin^2 \theta \right) \\
                                      & = \cot^2 \theta - \cos^2 \theta \\
        \end{align*}

      \item[60] 
        \begin{align*}
          \frac{1 + \sec^2 x}{1 + \tan^2 x} & = \frac{1 + \sec^2 x}{\sec^2 x} \\
                                            & = \frac{1}{\sec^2 x} + 1 \\
                                            & = 1 + \cos^2 x \\
        \end{align*}

      \item[61] 
        \begin{align*}
          \frac{\sec x}{\sec x - \tan x} & = \frac{\sec x}{\sfrac{1}{\cos x} - \sfrac{\sin x}{\cos x}} \\
                                         & = \frac{\sfrac{1}{\cos x}}{\sfrac{(1 - \sin x)}{\cos x}} \\
                                         & = \frac{1}{1 - \sin x} \\
                                         & = \frac{1 + \sin x}{(1 - \sin x)(1 + \sin x)} \\
                                         & = \frac{1 + \sin x}{1 - \sin^2 x} \\
                                         & = \frac{1 + \sin x}{\cos^2 x} \\
                                         & = \frac{1}{\cos^2 x} + \frac{\sin x}{\cos x} \cdot \frac{1}{\cos x} \\
                                         & = \sec^2 x + \sec x \tan x \\
                                         & = \sec x ( \sec x + \tan x ) \\
        \end{align*}

      \item[62] 
        \begin{align*}
          \frac{\sec x + \csc x}{\tan x + \cot x} & = \frac{\sfrac{1}{\cos x} + \sfrac{1}{\sin x}}{\sfrac{\sin x}{\cos x} + \sfrac{\cos x}{\sin x}} \\
              & = \frac{ \left( \cfrac{\sin x + \cos x}{\sin x \cos x} \right) }{\left( \cfrac{\sin^2 x + \cos^2 x}{\sin x \cos x} \right)} \\
              & = \frac{\sin x + \cos x}{\sin^2 x + \cos^2 x} \\
              & = \sin x + \cos x \\
        \end{align*}

      \item[63] 
        \begin{align*}
          \sec v - \tan v & = (\sec v - \tan v) \cdot \frac{\sec v + \tan v}{\sec v + \tan v} \\
                          & = \frac{\sec^2 v - \tan^2 v}{\sec v + \tan v} \\
                          & = \frac{1}{\sec v + \tan v} \\
        \end{align*}

      \item[64] 
        \begin{align*}
          \frac{\sin A}{1 - \cos A} & = \frac{\sin A}{1 - \cos A} \cdot \frac{1 + \cos A}{1 + \cos A} - \cot A \\
                                    & = \frac{\sin A ( 1 + \cos A )}{1 - \cos^2 A} - \cot A \\
                                    & = \frac{\sin A ( 1 + \cos A )}{\sin^2 A} - \cot A \\
                                    & = \frac{1 + \cos A}{\sin A} - \frac{\cos A}{\sin A} \\
                                    & = \frac{1}{\sin A} \\
                                    & = \csc A \\
        \end{align*}

      \item[70] 
        \begin{align*}
          \frac{\tan v \sin v}{\tan v + \sin v} & = \frac{\tan v \sin v}{\tan v + \sin v} \cdot \frac{\tan v - \sin v}{\tan v - \sin v} \\
                                                & = \frac{\tan v \sin v (\tan v - \sin v)}{\tan^2 v - \sin^2 v} \\
                                                & = \frac{\tan v \sin v (\tan v - \sin v)}{\sfrac{\sin^2 v}{\cos^2 v} - \sin^2 v} \\
                                                & = \frac{\tan v \sin v (\tan v - \sin v)}{\sin^2 v \left( \sfrac{1}{\cos^2 v} - 1 \right) } \\
                                                & = \frac{\tan v \sin v (\tan v - \sin v)}{\sin^2 v \left( \sec^2 v - 1 \right) } \\
                                                & = \frac{\tan v \sin v (\tan v - \sin v)}{\sin^2 v \tan^2 v } \\
                                                & = \frac{\tan v - \sin v}{\tan v \sin v } \\
        \end{align*}

    \end{description}

  \else
    \vspace{5 cm}

    \begin{quote}
      \begin{em}
        Our inventions are wont to be pretty toys, which distract our attention from serious things. They are but
        improved means to an unimproved end, an end which it was already but too easy to arrive at.
      \end{em}
    \end{quote}
    \hspace{1 cm} --Henry David Thoreau
  \fi

\end{document}

