\documentclass{exam}

\usepackage{units} 
\usepackage{graphicx}
\usepackage[fleqn]{amsmath}
\usepackage{cancel}
\usepackage{float}
\usepackage{mdwlist}
\usepackage{booktabs}
\usepackage{cancel}
\usepackage{polynom}
\usepackage{caption}
\usepackage{fullpage}
\usepackage{comment}
\usepackage{enumerate}
\usepackage{xfrac}
\usepackage{parskip}

\newcommand{\dg}{\ensuremath{^\circ}} 
\everymath{\displaystyle}

% \printanswers
\excludecomment{comment}

\ifprintanswers 
  \usepackage{2in1, lscape} 
\fi

\author{}
\date{December 17, 2014}
\title{Math 142 \\ Homework Fourteen}

\begin{document}

  \maketitle

  \section{Homework}
  Section 7.3: 1-2, 9-19, 23-30, 41-50, 61-64, 70-76

  \section{Extra Credit}
  Section 7.3: 89

  \ifprintanswers
    Since the angles form a triangle, they add up to $180 \dg$:
    \begin{align*}
      A + B + C & = 180 \dg \\
      C         & = 180 \dg - (A + B) \\
      \\
      \cos C & = \cos (180 \dg - (A + B)) \\
             & = \cos 180 \dg \cos (A + B) + \sin 180 \dg \sin (A + B) \\
             & = - \cos (A + B) \\
             & = \sin A \sin B - \cos A \cos B \\
             \\
      \cos A &= \sin B \sin C - \cos B \cos C \\
      \cos B &= \sin A \sin C - \cos A \cos C \\
      \\
      \sin (A + B) & = \sin (180 \dg - C) \\
                   & = \sin C \\
      \\
      \cos (A + B) & = \cos (180 \dg - C) \\
                   & = - \cos C \\
    \end{align*}

    Some other useful facts are:
    \begin{align*}
      \sin (A + B) &= \sin A \cos B + \cos A \sin B \\
      \\
      \cos (A + B)  & = \cos A \cos B - \sin A \sin B \\
      \cos A \cos B & = \cos (A + B) + \sin A \sin B \\
    \end{align*}
    
    \pagebreak

    You can substitute the above expressions at the appropriate spots to get to the desired final expression:
    \begin{align*}
      \sin 2A & + \sin 2B + \sin 2C  = 2 \sin A \cos A + 2 \sin B \cos B + 2 \sin C \cos C \\
              & = 2 \sin A ( \sin B \sin C - \cos B \cos C ) \\
                & \qquad{} + 2 \sin B ( \sin A \sin C - \cos A \cos C ) \\
                & \qquad{} + 2 \sin C ( \sin A \sin B - \cos A \cos B ) \\
              & = 6 \sin A \sin B \sin C  - 2 (\sin A \cos B \cos C \\
                & \qquad{} + \cos A \sin B \cos C + \cos A \cos B \sin C) \\
              & = 6 \sin A \sin B \sin C  - 2 ( \cos C ( \sin A \cos B + \cos A \sin B ) \\
                & \qquad{} + \cos A \cos B \sin C) \\
              & = 6 \sin A \sin B \sin C  - 2 ( \cos C \sin (A + B) + \cos A \cos B \sin C) \\
              & = 6 \sin A \sin B \sin C  - 2 ( \cos C \sin (A + B) \\
                & \qquad{} + ( \cos (A + B) + \sin A \sin B ) \sin C) \\
              & = 6 \sin A \sin B \sin C \\
                & \qquad{} - 2 ( \cos C \sin C + ( - \cos C + \sin A \sin B ) \sin C) \\
              & = 6 \sin A \sin B \sin C \\
                & \qquad{} - 2 ( \cos C \sin C  - \cos C \sin C + \sin A \sin B \sin C) \\
              & = 6 \sin A \sin B \sin C  - 2 \sin A \sin B \sin C \\
              & = 4 \sin A \sin B \sin C \\
    \end{align*}
  \fi

  % \section{Review}

  \ifprintanswers
    \pagebreak

    \section{Section 7.3}
    \begin{description}

      \item[1] 
        \begin{tabular}[H]{ccc}
          \toprule
          $\sin x$           & $\cos x$           & $\tan x$      \\
          $\sfrac{5}{13}$    & $\sfrac{12}{13}$   & $\sfrac{5}{12}$ \\
          \midrule
          $\sin 2x$          & $\cos 2x$          & $\tan 2x$      \\
          $\sfrac{120}{169}$ & $\sfrac{119}{169}$ & $\sfrac{120}{119}$ \\
          \bottomrule
        \end{tabular}

      \item[2] 
        \begin{tabular}[H]{ccc}
          \toprule
          $\sin x$          & $\cos x$         & $\tan x$      \\
          $\sfrac{4}{5}$    & $- \sfrac{3}{5}$ & $-\sfrac{4}{3}$ \\
          \midrule
          $\sin 2x$         & $\cos 2x$        & $\tan 2x$      \\
          $-\sfrac{24}{25}$ & $-\sfrac{7}{25}$ & $-\sfrac{24}{7}$ \\
          \bottomrule
        \end{tabular}

      \item[9]
        \begin{align*}
          \sin^4 x & = \left( \sin^2 x \right)^2 \\
                   & = \left( \frac{1 - \cos 2x}{2} \right)^2 \\
                   & = \frac{1 - 2 \cos 2x + \cos^2 2x}{4} \\
                   &= \frac{1}{4} - \frac{\cos 2x}{2} + \frac{\cos^2 2x}{4} \\
                   &= \boxed{ \frac{1}{4} - \frac{\cos 2x}{2} + \frac{1 + \cos 4x}{8} } \\
        \end{align*}

      \item[10]
        \begin{align*}
          \cos^4 x & = \left( \cos^2 x \right)^2 \\
                   & = \left( \frac{1 + \cos 2x}{2} \right)^2 \\
                   & = \frac{1 + 2 \cos 2x + \cos^2 2x}{4} \\
                   &= \frac{1}{4} + \frac{\cos 2x}{2} + \frac{\cos^2 2x}{4} \\
                   &= \boxed{ \frac{1}{4} + \frac{\cos 2x}{2} + \frac{1 + \cos 4x}{8} } \\
        \end{align*}

      \item[11]
        \begin{align*}
          \cos^2 x & \sin^4 x = \cos^2 x \left( \sin^2 x \right)^2 \\
                   & = \left( \frac{1 + \cos 2x}{2} \right) \left( \frac{1 - \cos 2x}{2} \right) \left( \frac{1 - \cos 2x}{2} \right) \\
                   & = \left( \frac{1 - \cos^2 2x}{4} \right) \left( \frac{1 - \cos 2x}{2} \right) \\
                   & = \frac{1 - \cos^2 2x - \cos 2x + \cos^3 2x}{8} \\
                   & = \frac{1}{8} \left( 1 - \frac{1 + \cos 4x}{2} - \cos 2x + \cos 2x \left( \frac{1 + \cos 4x}{2} \right) \right) \\
                   & = \frac{1}{8} \left( 1 - \frac{1}{2} - \frac{\cos 4x}{2} - \cos 2x + \frac{\cos 2x}{2} + \frac{\cos 2x \cos 4x}{2} \right) \\
                   & = \frac{1}{8} \left( \frac{1}{2} - \frac{\cos 2x}{2} - \frac{\cos 4x}{2} + \frac{\cos 2x \cos 4x}{2} \right) \\
                   & = \boxed{ \frac{1}{16} ( 1 - \cos 2x - \cos 4x + \cos 2x \cos 4x ) } \\
        \end{align*}

      \item[12]
        \begin{align*}
          \cos^4 x & \sin^2 x = \left( \cos^2 x \right)^2 \sin^2 x \\
                   & = \left( \frac{1 + \cos 2x}{2} \right) \left( \frac{1 + \cos 2x}{2} \right) \left( \frac{1 - \cos 2x}{2} \right) \\
                   & = \left( \frac{1 + \cos 2x}{4} \right) \left( \frac{1 - \cos^2 2x}{2} \right) \\
                   & = \frac{1}{8} \left( 1 - \cos^2 2x + \cos 2x - \cos^3 2x \right) \\
                   & = \frac{1}{8} \left( 1 + \cos 2x - \frac{1 + \cos 4x}{2}  - \frac{\cos 2x}{2} \left( \frac{1 + \cos 4x}{2} \right) \right) \\
                   & = \frac{1}{8} \left( 1 + \cos 2x - \frac{1}{2}  - \frac{\cos 4x}{2} - \frac{\cos 2x}{2} - \frac{\cos 2x \cos 4x}{2} \right) \\
                   & = \frac{1}{8} \left( \frac{1}{2} + \frac{\cos 2x}{2} - \frac{\cos 4x}{2}  - \frac{\cos 2x \cos 4x}{2} \right) \\
                   & = \boxed{ \frac{1}{16} \left( 1 + \cos 2x - \cos 4x  - \cos 2x \cos 4x \right) } \\
        \end{align*}

      \item[13]
        \begin{align*}
          \cos^4 x & \sin^4 x = \left( \frac{1 - \cos 2x}{2} \right)^2 \left( \frac{1 + \cos 2x}{2} \right)^2 \\
                   & = \left( \frac{1 - \cos^2 2x}{4} \right)^2 \\
                   & = \left( \frac{1}{8} - \frac{\cos 4x}{8} \right)^2 \\
                   & = \frac{1}{64} \left( 1 - \cos 4x \right)^2 \\
                   & = \frac{1}{64} \left( 1 - 2 \cos 4x + \cos^2 4x \right) \\
                   & = \frac{1}{64} \left( 1 - 2 \cos 4x + \frac{1 + \cos 8x}{2} \right) \\
                   & = \boxed{ \frac{1}{128} \left( 3 - 4 \cos 4x + \cos 8x \right) } \\
        \end{align*}

      \item[15]
        \begin{align*}
          \sin 15 \dg & = \sin \frac{30 \dg}{2} \\
                      & = \sqrt{  \frac{1 - \sfrac{\sqrt{3}}{2}}{2} } \\
                      & = \boxed{ \frac{1}{2} \sqrt{2 - \sqrt{3}} } \\
        \end{align*}

      \item[16]
        \begin{align*}
          \tan 15 \dg & = \tan \frac{30 \dg}{2} \\
                      & = \frac{ 1 - \sfrac{\sqrt{3}}{2} }{ \sfrac{1}{2} } \\
                      & = \boxed{ 2 - \sqrt{3} } \\
        \end{align*}

      \item[17]
        \begin{align*}
          \tan 22.5 \dg & = \tan \frac{45 \dg}{2} \\
                        & = \frac{1 - \sfrac{\sqrt{2}}{2}}{\sfrac{\sqrt{2}}{2}} \\
                        & = \boxed{ \sqrt{2} - 1 } \\
        \end{align*}

      \item[18]
        \begin{align*}
          \sin 75 \dg & = \sin \frac{150 \dg}{2} \\
                      & = \sqrt{ \frac{1 - (\sfrac{\sqrt{3}}{2})}{2} } \\
                      & = \boxed{ \frac{1}{2} \sqrt{2 + \sqrt{3}} } \\
        \end{align*}

      \item[19]
        Since $165 \dg$ is in Q-II, $\cos 165 \dg < 0$
        \begin{align*}
          \cos 165 \dg & = - \cos \frac{330 \dg}{2}  \\
                       & = - \sqrt{ \frac{1 + \sfrac{\sqrt{3}}{2}}{2} } \\
                       & = \boxed{ - \frac{1}{2} \sqrt{ 2 + \sqrt{3} } } \\
        \end{align*}

      \item[23]
        \begin{align*}
          \cos \frac{\pi}{12} & = \cos \frac{\sfrac{\pi}{6}}{2} \\
                              & = \sqrt{ \frac{1 + \sfrac{\sqrt{3}}{2}} {2} } \\
                              & = \boxed{ \frac{1}{2} \sqrt{2 + \sqrt{3}} } \\
        \end{align*}

      \item[24]
        \begin{align*}
          \tan \frac{5 \pi}{12} & = \tan \frac{\sfrac{5 \pi}{6}}{2} \\
                                & = \frac{ 1 - \left( - \sfrac{\sqrt{3}}{2} \right) }{\sfrac{1}{2}} \\
                                & = \boxed{ 2 + \sqrt{3} } \\
        \end{align*}

      \item[25]
        Since $\sfrac{9 \pi}{8}$ is in Q-III, $\sin \sfrac{9 \pi}{8} < 0$.
        \begin{align*}
          \sin \frac{9 \pi}{8} & = \sin \frac{\sfrac{9 \pi}{4}}{2} \\
                               & = - \sqrt{ \frac{1 - \sfrac{1}{\sqrt{2}}}{2} } \\
                               & = \boxed{ - \frac{1}{2} \sqrt{ 2 - \sqrt{2} } } \\
        \end{align*}

      \item[26]
        Since $\sfrac{11 \pi}{12}$ is in Q-II, $\sin \sfrac{11 \pi}{12} > 0$.
        \begin{align*}
          \sin \frac{11 \pi}{12} & = \sin \frac{\sfrac{11 \pi}{6}}{2} \\
                                 & = \sqrt{ \frac{1 - \sfrac{\sqrt{3}}{\sqrt{2}}}{2} } \\
                                 & = \boxed{ \frac{1}{2} \sqrt{ 2 - \sqrt{3} } } \\
        \end{align*}

      \item[27]
        \begin{parts}
          \part 
            \[
              2 \sin 18 \dg \cos 18 \dg = \boxed{ \sin 36 \dg }
            \]

          \part 
            \[
              2 \sin 3 \theta \cos 3 \theta = \boxed{ \sin 6 \theta }
            \]
        \end{parts}

      \item[28]
        \begin{parts}
          \part 
            \[
              \frac{2 \tan 7 \dg}{1 - \tan^2 7 \dg} = \boxed{ \tan 14 \dg }
            \]

          \part 
            \[
              \frac{2 \tan 7 \theta}{1 - \tan^2 7 \theta} = \boxed{ \tan 14 \theta }
            \]
        \end{parts}

      \item[29]
        \begin{parts}
          \part 
            \[
              \cos^2 34 \dg - \sin^2 34 \dg = \boxed{ \cos 68 \dg }
            \]

          \part 
            \[
              \cos^2 5 \theta  - \sin^2 5 \theta = \boxed{ \cos 10 \theta }
            \]
        \end{parts}

      \item[30]
        \begin{parts}
          \part 
            \[
              \cos^2 \frac{\theta}{2}  - \sin^2 \frac{\theta}{2} = \boxed{ \cos \theta }
            \]

            \[
              2 \sin \frac{\theta}{2} \cos \frac{\theta}{2} = \boxed{ \sin \theta }
            \]
        \end{parts}

      \item[41]
        \[
          \sin 2x \cos 3x = \boxed{ \frac{1}{2} \left[ \sin 5x - \sin x \right] }
        \]

      \item[42]
        \[
          \sin x \sin 5x = \boxed{ \frac{1}{2} \left[ \cos 4x - \cos 6x \right] }
        \]

      \item[43]
        \[
          \sin 4x \cos x = \boxed{ \frac{1}{2} \left[ \sin 5x + \sin 3x \right] } 
        \]

      \item[44]
        \[
          \cos 5x \cos 3x = \boxed{ \frac{1}{2} \left[ \cos 8x + \cos 2x \right] } 
        \]

      \item[45]
        \[
          3 \cos 4x \cos 7x = \boxed{ \frac{3}{2} \left[ \cos 11x + \cos 3x \right] } 
        \]

      \item[46]
        \[
          11 \sin \frac{x}{2} \cos \frac{x}{4} = \boxed{ \frac{11}{2} \left[ \cos \frac{3x}{4} + \cos \frac{x}{4} \right] } 
        \]

      \item[47]
        \begin{align*}
          \sin 5x + \sin 3x & = 2 \sin \frac{5x + 3x}{2} \cos \frac{5x - 3x}{2} \\
                            & = \boxed{ 2 \sin 4x \cos x } \\
        \end{align*}

      \item[48]
        \begin{align*}
          \sin x - \sin 4x & = 2 \cos \frac{x + 4x}{2} \sin \frac{x - 4x}{2} \\
                           & = - 2 \cos \frac{5x}{2} \sin \left( -\frac{3x}{2} \right) \\
                           & = \boxed{ 2 \cos \frac{5x}{2} \sin \frac{3x}{2} } \\
        \end{align*}

      \item[49]
        \begin{align*}
          \cos 4x - \cos 6x & = - 2 \sin \frac{4x + 6x}{2} \sin \frac{4x - 6x}{2} \\
                            & = -2 \sin 5x \sin (-x) \\
                            & = \boxed{ 2 \sin 5x \sin x } \\
        \end{align*}

      \item[50]
        \begin{align*}
          \cos 9x + \cos 2x & = 2 \cos \frac{9x + 2x}{2} \cos \frac{9x - 2x}{2} \\
                            & = \boxed{ 2 \cos \frac{11x}{2} \cos \frac{7x}{2} } \\
        \end{align*}

      \item[61]
        \begin{align*}
          (\sin x + \cos x)^2 & = \sin^2 x + 2 \sin x \cos x + \cos^2 x \\
                              & = 1 + 2 \sin x \cos x \\
                              & = 1 + \sin 2x \\
        \end{align*}

      \item[62]
        \begin{align*}
          \frac{2 \tan x}{1 + \tan^2 x} & = \frac{2 \sfrac{\sin x}{\cos x}}{1 + \sfrac{\sin^2 x}{\cos^2 x}} \\
                                        & = \frac{2 \sin x \cos x}{\cos^2 x + \sin^x x} \\
                                        & = 2 \sin x \cos x \\
                                        & = \sin 2x \\
        \end{align*}

      \item[63]
        \begin{align*}
          \frac{\sin 4x}{\sin x} & = \frac{2 \sin 2x \cos 2x}{\sin x} \\
                                 & = \frac{4 \sin x \cos x \cos 2x}{\sin x} \\
                                 & = 4 \cos x \cos 2x \\
        \end{align*}

      \item[64]
        \begin{align*}
          \frac{1 + \sin 2x}{\sin 2x} & = \frac{1}{\sin 2x} + 1 \\
                                      & = 1 + \frac{1}{2 \sin x \cos x} \\
                                      & = 1 + \frac{1}{2} \sec x \csc x \\
        \end{align*}

      \item[70]
        \begin{align*}
          \cos \left( x + \frac{\pi}{2} \right) & = \cos x \cos \frac{\pi}{2} - \sin x \sin \frac{\pi}{2} \\
                                                & = - \sin x \\
          \\
          \tan^2 \left( \frac{x}{2} + \frac{\pi}{4} \right) 
            &= \frac{1 - \cos \left( x + \sfrac{\pi}{2} \right)}{1 + \cos \left( x + \sfrac{\pi}{2} \right)} \\
            &= \frac{1 - (- \sin x)}{1 + (- \sin x)} \\
            &= \frac{1 + \sin x}{1 - \sin x} \\
        \end{align*}

      \item[71]
        \begin{align*}
          \frac{\sin x + \sin 5x}{\cos x + \cos 5x} & = \frac{2 \sin (3x) \cos (-2x)}{2 \cos(3x) \cos (-2x)} \\
                                                    & = \frac{\sin 3x}{\cos 3x} \\
                                                    & = \tan 3x \\
        \end{align*}

      \item[72]
        \begin{align*}
          \frac{\sin 3x + \sin 7x}{\cos x + \cos 5x} & = \frac{2 \sin 3x \cos 2x}{2 \cos3x \cos (2x)} \\
                                                    & = \frac{\sin 3x}{\cos 3x} \\
                                                    & = \tan 3x \\
        \end{align*}

      \item[73]
        \begin{align*}
          \frac{\sin 10x}{\sin 9x + \sin x} & = \frac{2 \sin 5x \cos 5x}{2 \sin 5x \sin 4x} \\
                                            & = \frac{\cos 5x}{\sin 4x} \\
        \end{align*}

      \item[74]
        \begin{align*}
          \frac{\sin x + \sin 3x + \sin 5x}{\cos x + \cos 3x + \cos 5x} & = \frac{\sin 3x + (\sin x + \sin 5x)}{\cos 3x + (\cos x + \cos 5x)} \\
                                                                        & = \frac{\sin 3x + 2 \sin 3x \cos 2x}{\cos 3x + 2 \cos 3x \cos 2x} \\
                                                                        & = \frac{\sin 3x (1 + 2 \cos 2x)}{\cos 3x (1 + 2 \cos 2x)} \\
                                                                        & = \frac{\sin 3x}{\cos 3x} \\
                                                                        & = \tan 3x \\
        \end{align*}

      \item[75]
        \begin{align*}
          \frac{\sin x + \sin x}{\cos x + \cos x} & = \frac{2 \sin \sfrac{(x + y)}{2} \cos \sfrac{(x - y)}{2}}{2 \cos \sfrac{(x + y)}{2} \cos \sfrac{(x - y)}{2}} \\
                                                  & = \frac{\sin \sfrac{(x + y)}{2}}{\cos \sfrac{(x + y)}{2}} \\
                                                  & = \tan \frac{x + y}{2} \\
        \end{align*}

      \item[76]
        \begin{align*}
          & \frac{\sin (x + y) - \sin (x - y)}{\cos (x + y) - \cos (x - y)} \\
            & = \frac{2 \cos \left( \cfrac{x + y + x - y}{2} \right) \sin \left( \cfrac{x + y - (x - y)}{2} \right)}
                     {2 \cos \left( \cfrac{x + y + x - y}{2} \right) \cos \left( \cfrac{x + y - (x - y)}{2} \right)} \\
            & = \frac{2 \cos x \sin y}{2 \cos x \cos y} \\
            & = \tan y \\
        \end{align*}

    \end{description}

  \else
    \vspace{9 cm}

    \begin{quote}
      \begin{em}
	For those who stubbornly seek freedom around the world, there can be no more
	urgent task than to come to understand the mechanisms and practices of
	indoctrination. These are easy to perceive in the totalitarian societies, much
	less so in the propaganda system to which we are subjected and in which all too
	often we serve as unwilling or unwitting instruments.
      \end{em}
    \end{quote}
    \hspace{1 cm} --Noam Chomsky
  \fi

\end{document}

